\section{Dynamics of zeroes}\label{dynamics-sec}

In this section we control the dynamics of the zeroes of $H_t$ in order to establish Theorem \ref{ubc-0}.  As $H_t$ is even with functional equation $H_t = H_t^*$, the zeroes are symmetric around the origin and the real axis; from \eqref{htdef} and the positivity of $\Phi$, we also see that $H_t(iy) > 0$ for all $y \in \R$, so there are no zeroes on the imaginary axis.  From the super-exponential decay of $\Phi$ and \eqref{htdef} we see that the entire function $H_t$ is of order $1$; by Jensen's formula, this implies that the number of zeroes in a large disk $D(0,R)$ is at most $O( R^{1+o(1)})$ as $R \to \infty$.

We begin with the analysis of the dynamics of a single zero of $H_t$:

\begin{proposition}[Dynamics of a single zero]\label{dynam}  Let $t_0 \in \R$, and let $(z_k(t_0))_{k \in \Z \backslash \{0\}}$ be an enumeration of the zeroes of $H_{t_0}$ in $\C$ (counting multiplicity), with the symmetry condition $z_{-k}(t_0) = -z_k(t_0)$.
\begin{itemize}
\item[(i)]  If $j \in \Z \backslash \{0\}$ is such that $z_j(t_0)$ is a simple zero of $H_{t_0}$, then there exists a neighbourhood $U$ of $z_j(t_0)$, a neighbourhood $I$ of $t_0$ in $\R$, and a smooth map $z_j: I \to U$ such that for every $t \in I$, $z_j(t)$ is the unique zero of $H_t$ in $U$.  Furthermore one has the equation
\begin{equation}\label{zjk}
 \frac{\partial z_j}{\partial t}(t_0) = 2 \sum^{\prime}_{k \neq j} \frac{1}{z_j(t_0) - z_k(t_0)} 
\end{equation}
where the sum is over those $k \in \Z \backslash \{0\}$ with $k \neq j$, and the prime means that the $k$ and $-k$ terms are summed together (except for the $k=-j$ term, which is summed separately) in order to make the sum convergent.
\item[(ii)]  If $j \in \Z \backslash \{0\}$ is such that $z_j(t_0)$ is a repeated zero of $H_{t_0}$ of order $m \geq 2$, then there is a neighbourhood $U$ of $z_j(t_0)$ such that for $t$ sufficiently close to $t_0$, there are precisely $m$ zeroes of $H_t$ in $U$, and they take the form
$$ z_j(t_0) + \sqrt{2} (t-t_0)^{1/2} x_j + O( |t-t_0|)$$
for $j=1,\dots,m$ as $t \to t_0$, where $x_1 < \dots < x_m$ are the roots of the $m^{\operatorname{th}}$ Hermite polynomial
\begin{align}
\operatorname{He}_m(z) &\coloneqq (-1)^m \exp\left(\frac{z^2}{2}\right) \frac{d^m}{dz^m} \exp\left(-\frac{z^2}{2}\right)\label{heform}\\
&= \sum_{0 \leq l \leq m/2} \frac{m!}{l! (m-2l)!} (-1)^l \frac{z^{m-2l}}{2^l}\label{heform2}
\end{align}
and the implied constant in the $O()$ notation can depend on $t_0$, $j$, and $m$.
\end{itemize}
\end{proposition}

The differential equation \eqref{zjk} was previously derived in \cite[Lemma 2.4]{csv} in the case $t > \Lambda$ (in which all zeroes are real and simple); however, in our applications we also need to consider the regime $t \leq \Lambda$ in which the zeroes are permitted to be complex or repeated.
The roots $x_1,\dots,x_m$ appearing in Proposition \ref{heform}(ii) can be given explicitly for small values of $m$ as
$$ x_1 = -1; \quad x_2 = +1$$
when $m=2$,
$$ x_1 = -\sqrt{3}; \quad x_2 = 0; \quad x_3 = +\sqrt{3}$$
when $m=3$, and
$$ x_1 = -\sqrt{3+\sqrt{6}}; \quad x_2 = -\sqrt{3-\sqrt{6}}; \quad x_3 = \sqrt{3 - \sqrt{6}}; \quad  x_4 = \sqrt{3 + \sqrt{6}}$$
when $m=4$.  From \eqref{heform} and iterating Rolle's theorem we see that all the roots $x_1,\dots,x_m$ of $\operatorname{He}_m$ are real; from the Hermite equation $\left(\frac{d^2}{dz^2} - z \frac{d}{dz} + m\right) \operatorname{He}_m(z) = 0$ and the Picard uniqueness theorem for ODE we see that the zeroes are all simple.

\begin{proof}  First suppose we are in the situation of (i).  As $z_j(t_0)$ is simple, $\frac{\partial}{\partial z} H_t$ is non-zero at $z_j(t_0)$; since $H_t(z)$ is a smooth function of both $t$ and $z$, we conclude from the implicit function theorem that there is a unique solution $z_j(t) \in U$ to the equation
$$ H_t( z_j(t) ) = 0$$
with $z_j(t)$ in a sufficiently small neighbourhood $U$ of $z_j(t_0)$, if $t$ is in a sufficiently small neighbourhood $I$ of $t_0$; furthermore, $z_j(t)$ depends smoothly on $t$, and agrees with $z_j(t_0)$ when $t=t_0$.  Differentiating the above equation at $t_0$, we obtain
$$ \frac{\partial H_t}{\partial t}|_{t=t_0}( z_j(t_0) ) + \frac{\partial z_j}{\partial t}(t_0) H'_{t_0}(z_j(t_0)) = 0,$$
where the primes denote differentiation in the $z$ variable.
On the other hand, from \eqref{htdef} and differentiation under the integral sign (which can be justified using the rapid decrease of $\Phi$) we have the backwards heat equation
\begin{equation}\label{back}
\frac{\partial H_t}{\partial t} = -H''_t
\end{equation}
for all $t \geq 0$.  Inserting this into the previous equation, we conclude that
\begin{equation}\label{tzj}
\frac{\partial z_j}{\partial t}(t_0)  = \frac{H''_t}{H'_t}( z_j(t_0) ),
\end{equation}
noting that the denominator $H'_t(z_j(t_0))$ is non-vanishing by the hypothesis that the zero at $z_j(t_0)$ is simple.  Henceforth we omit the dependence on $t_0$ for brevity.  From Taylor expansion of $H_t$, $H'_t$, and $H''_t$ around the simple zero $z_j$ we see that
\begin{equation}\label{htz-eq}
 \frac{H''_t}{H'_t}( z_j) = 2 \lim_{z \to z_j}\left(  \frac{H'_t}{H_t}( z) - \frac{1}{z-z_j} \right).
\end{equation}
On the other hand, as $H_t$ is even, non-zero at the origin (as follows from \eqref{htdef} and the positivity of $\Phi$), and entire of order $1$, we see from the Hadamard factorization theorem that
$$ H_t(z) = H_t(0) \prod_k^{\prime} \left(1 - \frac{z}{z_k}\right),$$
where the prime indicates that the $k$ and $-k$ factors are multiplied together.  The product is locally uniformly convergent, so we may take logarithmic derivatives and conclude that
$$ \frac{H'_t}{H_t}(z) = \sum_k^{\prime} \frac{1}{z-z_k}.$$
Inserting this into \eqref{tzj}, \eqref{htz-eq} and using the continuity of $z \mapsto \sum_{k: k \neq j}^\prime \frac{1}{z-z_k}$ at $z_j$ (which follows from the growth in the number of zeroes, either from the dominated convergence theorem or the Weierstrass $M$-test), we obtain the claim (i).

Now we prove (ii).  We abbreviate $z_j(t_0)$ as $z_j$.  By Taylor expansion we have
$$ \frac{\partial^{2k} H_{t_0}}{\partial z^{2k}}(z) = m (m-1) \dots (m-2k+1) a_m (z-z_j)^{m-2k} + O( |z-z_j|^{\max(m-2k+1,0)} )$$
as $z \to z_j$ for any fixed integer $k \geq 0$ and some non-zero complex number $a_m = a_m(z_j, t_0)$ (with the implied constant in the $O()$ notation allowed to depend on $k$, $z_j$, $t_0$); applying the backwards heat equation \eqref{back} we thus have
$$ \frac{\partial^k H_t}{\partial t^k}|_{t=t_0}(z) = (-1)^k m (m-1) \dots (m-2k+1) a_m (z-z_j)^{m-2k} + O( |z-z_j|^{\max(m-2k+1,0)} ).$$
Performing Taylor expansion in time and using \eqref{heform2}, we conclude that in the regime $z - z_j = O( |t-t_0|^{1/2} )$, one has the bound
$$ H_t(z) = a_m ((t-t_0)^{1/2})^m \left( \operatorname{He}_m\left( \sqrt{2} \frac{z-z_j}{(t-t_0)^{1/2}} \right) + O\left( |t-t_0|^{1/2} \right) \right)$$
as $t \to t_0$, using (say) the standard branch of the square root.  By the inverse function theorem (and the simple nature of the zeroes of $\operatorname{He}_m$), we conclude that for $t$ sufficiently close but not equal to to $t_0$, we have $m$ zeroes of $H_t$ of the form
$$ z_j + (t-t_0)^{1/2} x_j + O( |t-t_0| ).$$
By Rouche's theorem, if $U$ is a sufficiently small neighborhood of $z_j$ then these are the only zeroes of $H_t$ in $U$ for $t$ sufficiently close to $t_0$.  The claim follows.
\end{proof}

Next, we recall the following bound of de Bruijn:

\begin{theorem}\label{debr-bound}  Suppose that $t_0 \in \R$ and $y_0 > 0$ is such that there are no zeroes $H_{t_0}(x+iy)=0$ with $x \in \R$ and $y > y_0$.  Then for any $t>t_0$, there are no zeroes $H_{t}(x+iy)=0$ with $x \in \R$ and $y > \max( y_0^2 - 2(t-t_0), 0)^{1/2}$.  In particular one has $\Lambda \leq t_0 + \frac{1}{2} y_0^2$.
\end{theorem}

\begin{proof} See \cite[Theorem 13]{debr}.
\end{proof}

We are now ready to prove Theorem \ref{ubc-0}.  The main step is to establish

\begin{proposition}[Zero-free region criterion]\label{ubc}  Suppose that $t_0, X > 0$ and $0 < y_0 \leq 1$ obey the following hypotheses:
\begin{itemize}
\item[(i)]  There are no zeroes $H_0(x+iy)=0$ with $0 \leq x \leq X$ and $\sqrt{y_0^2+2 t_0} \leq y \leq 1$.
\item[(ii)]  There are no zeroes $H_{t_0}(x+iy)=0$ with $x \geq X+\sqrt{1-y_0^2}$ and $y_0 \leq y \leq \sqrt{1-2t_0}$.
\item[(iii)]  There are no zeroes $H_{t}(x+iy)=0$ with $X \leq x \leq X+\sqrt{1-y_0^2}$, $\sqrt{y_0^2 + 2(t_0-t)} \leq y \leq \sqrt{1-2t}$, and $0 \leq t \leq t_0$.
\end{itemize}
Then there are no zeroes $H_{t_0}(x+iy) = 0$ with $x \in \R$ and $y \geq y_0$.
\end{proposition}

\begin{proof}  It is well known that the Riemann $\xi$ function has no zeroes outside of the strip $\{ 0 \leq \mathrm{Re}(s) \leq 1 \}$, hence there are no zeroes $H_0(x+iy)=0$ with $y > 1$.  By Theorem \ref{debr-bound}, we may thus remove the upper bound constraints $y \leq 1$, $y \leq \sqrt{1-2t_0}$, and $y \leq \sqrt{1-2t}$ from (i), (ii), and (iii) respectively.

By hypotheses (ii), (iii) and the symmetry properties of $H_t$, it suffices to show that for every $0 \leq t \leq t_0$, there are no zeroes $H_t(x+iy) = 0$ with $0 \leq x \leq X$ and $y \geq Y(t)$, where $Y(t) \coloneqq \sqrt{y_0^2 + 2(t_0-t)}$.  By hypothesis (i), this is true at time $t=0$.  Suppose the claim failed for some time $0 < t \leq t_0$.  Let $t_1 \in (0,t_0]$ be the minimal time in which this occurred (such a time exists because $H_t$ varies continuously in $t$, and there are no zeroes $H_t(x+iy)=0$ with (say) $y>1$).  From Rouche's theorem (or Proposition \ref{dynam}) we conclude that there is a zero $H_{t_1}(x+iy)=0$ with $x+iy$ on the boundary of the region $\{ x+iy: 0 \leq	 x \leq X, y \geq Y(t_1) \}$.  The right side $x=X$ of this boundary is ruled out by hypothesis (ii), and (as mentioned at the start of the section) the left side $x=0$ is ruled out by \eqref{htdef} and the positivity of $\Phi$.  Thus by the symmetry properties of $H_{t_1}$ we must have
$$ H_{t_1}(x+iY(t_1)) = 0$$
for some $0 < x < X$.

Suppose first that $H_{t_1}$ has a repeated zero at $x+iy_0$.  Using Proposition \ref{dynam}(ii) and observing (from the symmetry of $\operatorname{He}_m$) that at least one of the roots $x_1,\dots,x_m$ is positive, we then see that for $t<t_1$ sufficiently close to $t_1$, $H_t$ has a zero in the region $\{ x+iy: 0 \leq x \leq X, y \geq Y(t) \}$, contradicting the minimality of $t_1$.  Thus the zero $x+i Y(t_1)$ of $H_{t_1}$ must be simple.  In particular, by Proposition \ref{dynam}(i) we can write $x+i Y(t_1) = z_j(t_1)$ for some smooth function $z_j$ in a neighbourhood of $t_1$ obeying \eqref{zjk}, such that $z_j(t)$ is a zero of $H_t$ for all $t$ close to $t_1$.  We will prove that
\begin{equation}\label{im}
\mathrm{Im} \frac{\partial}{\partial t} z_j( t_1 ) < \frac{\partial}{\partial t} Y(t_1),
\end{equation}
which implies that there is a zero of $H_t$ in the region $\{ x+iy: 0 \leq x \leq X, y \geq Y(t) \}$  for $t<t_1$ sufficiently close to $t_1$, giving the required contradiction.  

The right-hand side of \eqref{im} is
$$ \frac{\partial}{\partial t} Y(t_1) = -\frac{1}{Y(t_1)}.$$
By Proposition \ref{dynam}(i), the left-hand side of \eqref{im} is
$$ 2 \sum_{k \neq j}^{\prime} \frac{Y(t_1) - y_k}{(x-x_k)^2 + (Y(t_1)-y_k)^2}$$
where we write $z_k = x_k + i y_k$.  Clearly any zero $x_k+iy_k$ with imaginary part $y_k$ in $[-Y(t_1),Y(t_1)]$ gives a non-positive contribution to this sum, the contribution of the zero $x- iY(t_1)$ is $-\frac{1}{Y(t_1)}$, the contribution of the zero $-x+iY(t_1)$ vanishes, and the contribution of $-x-iY(t_1)$ is negative.  Grouping the remaining zeroes with their complex conjugates, it then suffices to show that
$$ \frac{Y(t_1) - y_k}{(x-x_k)^2 + (y_j-y_k)^2} + \frac{Y(t_1) + y_k}{(x-x_k)^2 + (Y(t_1)+y_k)^2} \leq 0$$
whenever $y_k > Y(t_1)$.  Cross-multiplying and canceling like terms, this inequality eventually simplifies to
$$ y_k^2 \leq (x-x_k)^2 + Y(t_1)^2.$$
But from the hypothesis (iii) and the assumption $y_k > Y(t_1)$, we have $|x_k| \geq X+\sqrt{1-Y(t_1)^2}$, so $(x-x_k)^2 \geq 1-Y(t_1)^2$.  On the other hand from Theorem \ref{debr-bound} one has $y_k < 1$, giving the required contradiction.
\end{proof}

By combining Proposition \ref{ubc} with Theorem \ref{debr-bound}, we obtain Theorem \ref{ubc-0}, noting from \eqref{hoz}, \eqref{sas} that condition (i) of Proposition \ref{ubc} is equivalent to condition (i) of Theorem \ref{debr-bound}.
